formal/inference/Trace_Matches.thy
@@ -1,18 +1,18 @@
 theory Trace_Matches
 imports Inference
 begin
-datatype io = I | O
-type_synonym index = "nat \<times> io \<times> nat"
+datatype ioTag = In | Out
+type_synonym index = "nat \<times> ioTag \<times> nat"
 
 fun lookup :: "index \<Rightarrow> execution \<Rightarrow> value" where
-  "lookup (eventNo, I, inx) t = (let (_, inputs, _) = nth t eventNo in nth inputs inx)" |
-  "lookup (eventNo, io.O, inx) t = (let (_, _, outputs) = nth t eventNo in nth outputs inx)"
+  "lookup (eventNo, In, inx) t = (let (_, inputs, _) = nth t eventNo in nth inputs inx)" |
+  "lookup (eventNo, Out, inx) t = (let (_, _, outputs) = nth t eventNo in nth outputs inx)"
 
 abbreviation eventNum :: "index \<Rightarrow> nat" where
   "eventNum i \<equiv> fst i"
 
-abbreviation io :: "index \<Rightarrow> io" where
-  "io i \<equiv> fst (snd i)"
+abbreviation ioTag :: "index \<Rightarrow> ioTag" where
+  "ioTag i \<equiv> fst (snd i)"
 
 abbreviation inx :: "index \<Rightarrow> nat" where
   "inx i \<equiv> snd (snd i)"
@@ -20,9 +20,32 @@ abbreviation inx :: "index \<Rightarrow> nat" where
 definition get_intratrace_matches :: "execution \<Rightarrow> (index \<times> index) fset" where
   "get_intratrace_matches e = Abs_fset {(a, b). lookup a e = lookup b e \<and> eventNum a \<le> eventNum b}"
 
+primrec index :: "value list \<Rightarrow> nat \<Rightarrow> ioTag \<Rightarrow> nat \<Rightarrow> index fset" where
+  "index [] _ _ _ = {||}" |
+  "index (h#t) eventNo io ind = finsert (eventNo, io, ind) (index t eventNo io (ind + 1))"
+
+definition io_index :: "nat \<Rightarrow> value list \<Rightarrow> value list \<Rightarrow> index fset" where
+  "io_index eventNo inputs outputs = (index inputs eventNo In 0) |\<union>| (index outputs eventNo Out 0)"
+
+definition indices :: "execution \<Rightarrow> index fset" where
+  "indices e = foldl (|\<union>|) {||} (map (\<lambda>(eventNo, (label, inputs, outputs)). io_index eventNo inputs outputs) (enumerate 0 e))"
+
+definition get_intratrace_matches_alt :: "execution \<Rightarrow> (index \<times> index) fset" where
+  "get_intratrace_matches_alt e = ffilter (\<lambda>(a, b). lookup a e = lookup b e \<and> eventNum a \<le> eventNum b \<and> a \<noteq> b) (indices e |\<times>| indices e)"
+
+lemma get_intratrace_matches_preproces:  "get_intratrace_matches_alt e = ffilter (\<lambda>(a, b). lookup a e = lookup b e) (ffilter (\<lambda>(a, b). eventNum a \<le> eventNum b \<and> a \<noteq> b) (indices e |\<times>| indices e))"
+  apply (simp add: get_intratrace_matches_alt_def)
+  apply (simp add: ffilter_def fset_both_sides Abs_fset_inverse fprod_def)
+  apply (simp add: Set.filter_def)
+  by auto
+
 primrec get_all_intratrace_matches :: "log \<Rightarrow> (index \<times> index) fset list" where
   "get_all_intratrace_matches [] = []" |
   "get_all_intratrace_matches (h#t) = (get_intratrace_matches h)#(get_all_intratrace_matches t)"
+
+primrec get_all_intratrace_matches_alt :: "log \<Rightarrow> (index \<times> index) fset list" where
+  "get_all_intratrace_matches_alt [] = []" |
+  "get_all_intratrace_matches_alt (h#t) = (get_intratrace_matches_alt h)#(get_all_intratrace_matches_alt t)"
 
 (* 
   To detect all intertrace matches, walk the trace in the current machine and replace eventNo with
